\[
  n_1
  =
  \frac{
    \rho
  }{
    2 - \rho
  }
  \addtag
\]

\[
  n_k^{(g)}
  =
  \frac{1}{\rho t}
  N_{k t}
  =
  \frac{1}{\rho}
  n_k
  \addtag
\]

Solving for $n_2^{(g)}$,

\[
  \frac{
    n_k
  }{
    n_{k-1}
  }
  =
  \frac{
    (k - 1)(1 - \rho)
  }{
    1 + (1 - \rho)k
  }
  \addtag
\]

\[
  n_k
  =
  \frac{
    (k - 1)(1 - \rho)
  }{
    1 + (1 - \rho)k
  }
  n_{k-1}
  \addtag
\]

\[
  n_2
  =
  \frac{
    (2 - 1)(1 - \rho)
  }{
    1 + (1 - \rho)2
  }
  n_1
  \addtag
\]

\[
  n_2
  =
  \frac{
    (1 - \rho)
  }{
    1 + 2(1 - \rho)
  }
  \left[
    \frac{
      \rho
    }{
      2 - \rho
    }
    \right]
  \addtag
\]

\[
  n_2^{(g)}
  =
  \frac{1}{\rho}
  n_2
  =
  \frac{1}{\rho}
  \left[
    \frac{
      1 - \rho
    }{
      3 - 2\rho
    }
  \right]
  \left[
    \frac{
      \rho
    }{
      2 - \rho
    }
  \right]
  \addtag
\]

\[
  n_2^{(g)}
  =
  \frac{
    (1 - \rho)
  }{
    (2 - \rho)
    (3 - 2\rho)
  }
  \addtag
\]

Now for $n_3^{(g)}$,

\[
  n_k
  =
  \frac{
    (k - 1)(1 - \rho)
  }{
    1 + (1 - \rho)k
  }
  n_{k-1}
  \addtag
\]

\[
  n_3
  =
  \frac{
    (3 - 1)(1 - \rho)
  }{
    1 + (1 - \rho)3
  }
  n_{2}
  \addtag
\]

\[
  n_3
  =
  \frac{
    2(1 - \rho)
  }{
    4 - 3\rho
  }
  \left[
    \frac{
    (1 - \rho)
  }{
    3 - 2\rho
  }
  \right]
  \left[
    \frac{
      \rho
    }{
      2 - \rho
    }
  \right]
  \addtag
\]

\[
  n_3^{(g)}
  =
  \frac{1}{\rho t}
  N_{3 t}
  =
  \frac{1}{\rho}
  n_3
  \addtag
\]

\[
  n_3^{(g)}
  =
  \frac{1}{\rho}
  \left[
    \frac{
      2(1 - \rho)
    }{
      4 - 3\rho
    }
  \right]
  \left[
    \frac{
    (1 - \rho)
  }{
    3 - 2\rho
  }
  \right]
  \left[
    \frac{
      \rho
    }{
      2 - \rho
    }
  \right]
  \addtag
\]

\[
  n_3^{(g)}
  =
  \frac{
    2 (1 - \rho)^2
  }{
    (4 - 3\rho)
    (3 - 2\rho)
    (2 - \rho)
  }
\]